src/Specific/NewBaseSystemTest.v
@@ -1,0 +1,128 @@
+Require Import Coq.ZArith.ZArith Coq.ZArith.BinIntDef.
+Require Import Coq.Lists.List. Import ListNotations.
+Require Import Crypto.NewBaseSystem. Import B.
+Require Import Crypto.ModularArithmetic.PrimeFieldTheorems.
+Require Import Crypto.Util.Tactics Crypto.Util.Decidable.
+Require Import Crypto.Util.LetIn.
+Require Crypto.Util.Tuple.
+Local Notation tuple := Tuple.tuple.
+Local Open Scope list_scope.
+Local Open Scope Z_scope.
+Local Coercion Z.of_nat : nat >-> Z.
+
+(*** 
+Modulus : 2^255-19
+Base: 25.5
+Comparison : F
+***)
+Section Ops.
+  Local Infix "^" := tuple : type_scope.
+
+  (* These `Let`s will need to be passed as Ltac arguments (or cleverly inferred *)
+  Let wt := fun i : nat => 2^(25 * (i / 2) + 26 * ((i + 1) / 2)).
+  Let sz := 10%nat.
+  Let s : Z := 2^255.
+  Let c : list B.limb := [(1, 19)].
+  Let coef_div_modulus := 2. (* add 2*modulus before subtracting *)
+  Let carry_chain := (seq 0 sz) ++ ([0;1])%nat.
+
+  (* These `Lets` are inferred from those above *)
+  Let m := Eval compute in Z.to_pos (s - Associational.eval c). (* modulus *)
+  Let sz2 := Eval compute in ((sz * 2) - 1)%nat.
+  Let coef := Eval vm_compute in (@Positional.encode wt modulo div sz (coef_div_modulus * (s-Associational.eval c))). (* subtraction coefficient *)
+  Let coef_mod : mod_eq m (Positional.eval (n:=sz) wt coef) 0 := eq_refl.
+
+  Definition zero_sig :
+    { zero : Z^sz | Positional.Fdecode (m:=m) wt zero = 0%F}.
+  Proof.
+    let t := eval vm_compute in
+    (Positional.encode (n:=sz) (modulo:=modulo) (div:=div) wt 0) in
+        exists t; vm_decide.
+  Defined.
+
+  Definition one_sig :
+    { one : Z^sz | Positional.Fdecode (m:=m) wt one = 1%F}.
+  Proof.
+    let t := eval vm_compute in
+    (Positional.encode (n:=sz) (modulo:=modulo) (div:=div) wt 1) in
+        exists t; vm_decide.
+  Defined.
+
+  Definition add_sig :
+    { add : (Z^sz -> Z^sz -> Z^sz)%type |
+               forall a b : Z^sz,
+                 let eval := Positional.Fdecode (m:=m) wt in
+                 eval (add a b) = (eval a  + eval b)%F }.
+  Proof.
+    eexists; cbv beta zeta; intros; assert_preconditions.
+    let x := constr:(
+        Positional.add_cps (n := sz) wt a b id) in
+    solve_op_F wt x. reflexivity.
+  Defined.
+
+  Definition sub_sig :
+    {sub : (Z^sz -> Z^sz -> Z^sz)%type |
+               forall a b : Z^sz,
+                 let eval := Positional.Fdecode (m:=m) wt in
+                 eval (sub a b) = (eval a - eval b)%F}.
+  Proof.
+    eexists; cbv beta zeta; intros; assert_preconditions.
+    let x := constr:(
+         Positional.sub_cps (n:=sz) (coef := coef) wt a b id) in
+    solve_op_F wt x. reflexivity.
+  Defined.
+
+  Definition opp_sig :
+    {opp : (Z^sz -> Z^sz)%type |
+               forall a : Z^sz,
+                 let eval := Positional.Fdecode (m := m) wt in
+                 eval (opp a) = F.opp (eval a)}.
+  Proof.
+    eexists; cbv beta zeta; intros; assert_preconditions.
+    let x := constr:(
+         Positional.opp_cps (n:=sz) (coef := coef) wt a id) in
+    solve_op_F wt x. reflexivity.
+  Defined.
+  
+  Definition mul_sig :
+    {mul : (Z^sz -> Z^sz -> Z^sz)%type |
+               forall a b : Z^sz,
+                 let eval := Positional.Fdecode (m := m) wt in
+                 eval (mul a b) = (eval a  * eval b)%F}.
+  Proof.
+    eexists; cbv beta zeta; intros; assert_preconditions.
+    let x := constr:(
+         Positional.mul_cps (n:=sz) (m:=sz2) wt a b
+           (fun ab => Positional.reduce_cps (n:=sz) (m:=sz2) wt s c ab id)) in
+    solve_op_F wt x. reflexivity.
+
+    (* rough breakdown of synthesis time *)
+    (* 1.2s for side conditions -- should improve significantly when [chained_carries] gets a correctness lemma *)
+    (* basesystem_partial_evaluation_RHS (primarily vm_compute): 1.8s, which gets re-computed during defined *)
+
+    (* doing [cbv -[Let_In runtime_add runtime_mul]] took 37s *)
+
+  Defined. (* 3s *)
+
+  (* Performs a full carry loop (as specified by carry_chain) *)
+  Definition carry_sig :
+    {carry : (Z^sz -> Z^sz)%type |
+               forall a : Z^sz,
+                 let eval := Positional.Fdecode (m := m) wt in
+                 eval (carry a) = eval a}.
+  Proof.
+    eexists; cbv beta zeta; intros; assert_preconditions.
+    let x := constr:(
+               Positional.chained_carries_cps (n:=sz) (div:=div)(modulo:=modulo) wt a carry_chain id) in
+    solve_op_F wt x. reflexivity.
+  Defined.
+
+End Ops.
+
+(*
+Eval cbv [proj1_sig add_sig] in (proj1_sig add_sig).
+Eval cbv [proj1_sig sub_sig] in (proj1_sig sub_sig).
+Eval cbv [proj1_sig opp_sig] in (proj1_sig opp_sig).
+Eval cbv [proj1_sig mul_sig] in (proj1_sig mul_sig).
+Eval cbv [proj1_sig carry_sig] in (proj1_sig carry_sig).
+*)
